day 12 part1

problems/12/Problem12.dfy
@@ -1,6 +1,185 @@
+include "../../parser/split.dfy"
+include "../../parser/parseInt.dfy"
+include "./QuickUnion.dfy"
 module Problem12 {
-    method problem12_1(input: string) returns (x: int) {
-        return 3;
+    import opened Split
+    import opened ParseInt
+    import opened Std.Collections.Seq
+    import opened QuickUnion
+    method parseInput(input: string) returns (data: seq<string>, dim: (nat, nat))
+        ensures |data| > 0
+        ensures dim.1 > 0
+        ensures dim.0 > 0
+        ensures dim.1 == |data|
+        ensures forall x :: x in data ==> |x| == dim.0
+    {
+        data := [];
+        var lines := splitOnBreak(input);
+        expect |lines| > 0;
+        expect |lines[0]| > 0;
+        dim := (|lines[0]|, |lines|-1);
+        expect dim.1 > 0;
+        for i := 0 to |lines| 
+            invariant forall x :: x in data ==> |x| == dim.0
+        {
+            if lines[i] != "" {
+                expect |lines[i]| == dim.0;
+                data := data + [lines[i]];
+            }
+        }
+        expect |data| == |lines|-1;
+        expect |data| > 0;
+    }
+
+    function pairToIndex(p: (nat, nat), dim: (nat, nat)): nat
+        requires dim.0 > 0
+        requires dim.1 > 0
+        requires 0 <= p.0 < dim.0
+        requires 0 <= p.1 < dim.1
+    {
+        p.0 + p.1 * dim.0
+    }
+
+    lemma pairToIndexLess(p: (nat, nat), dim: (nat, nat))
+        requires dim.0 > 0
+        requires dim.1 > 0
+        requires 0 <= p.0 < dim.0
+        requires 0 <= p.1 < dim.1
+        ensures pairToIndex(p, dim) < dim.0 * dim.1
+        decreases p.1
+    {
+        if p.1 == 0 {
+            assert pairToIndex(p, dim) < dim.0 * dim.1;
+        } else {
+            calc {
+                pairToIndex(p, dim);
+                p.0 + p.1 * dim.0;
+                p.0 + p.1 * dim.0 - dim.0 + dim.0;
+                p.0 + (p.1 - 1) * dim.0 + dim.0;
+                pairToIndex((p.0, p.1 - 1), dim) + dim.0;
+            }
+            pairToIndexLess((p.0, p.1 - 1), (dim.0, dim.1-1));
+            assert pairToIndex(p, dim) < dim.0 * dim.1;
+        }
+    }
+
+    function indexToPair(i: nat, dim: (nat, nat)): (nat, nat)
+        requires dim.0 > 0
+        requires dim.1 > 0
+        requires i < dim.0 * dim.1
+        ensures 0 <= indexToPair(i, dim).0 < dim.0
+        ensures 0 <= indexToPair(i, dim).1 < dim.1
+    {
+        assert i / dim.0 < dim.1 by {
+            if i / dim.0 >= dim.1 {
+                calc{
+                    dim.0*(i / dim.0);
+                    i;
+                }
+                assert false;
+            }
+        }
+        (i % dim.0, i / dim.0)
+    }
+
+    lemma ThereIsAMinimum(s: set<nat>)
+        requires s != {}
+        ensures exists x :: x in s && forall y :: y in s ==> x <= y
+    {
+        assert s != {};
+        var x :| x in s;
+        if s == {x} {
+        } else {
+            var s' := s - {x};
+            assert s == s' + {x};
+            ThereIsAMinimum(s');
+        }
+    }
+
+    function SetToSequence(s: set<nat>): seq<nat>
+        ensures var q := SetToSequence(s); forall i :: 0 <= i < |q| ==> q[i] in s
+        ensures |SetToSequence(s)| == |s|
+        ensures forall p :: p in s ==> p in SetToSequence(s)
+    {
+    if s == {} then [] else
+        ThereIsAMinimum(s);
+        var x :| x in s && forall y :: y in s ==> x <= y;
+        [x] + SetToSequence(s - {x})
+    }
+
+    method problem12_1(input: string) returns (x: int) 
+        decreases *
+    {
+        var data, dim := parseInput(input);
+        var union := new QuickUnion(dim.0 * dim.1);
+        x := 0;
+        assert union.n == dim.0 * dim.1;
+        assert union.parent.Length == dim.0 * dim.1;
+        assert fresh(union);
+        assert union.Valid();
+        for i := 0 to dim.1 
+            invariant union.n == dim.0 * dim.1
+            invariant union.Valid()
+            modifies  union.size, union.parent
+        {
+            for j := 0 to dim.0
+                invariant union.n == dim.0 * dim.1
+                invariant union.Valid()
+                modifies  union.size, union.parent
+            {
+                if i+1 < dim.1 && data[i][j] == data[i+1][j] {
+                    pairToIndexLess((j,i), dim);
+                    pairToIndexLess((j,i+1), dim);
+                    assert union.parent.Length == dim.0 * dim.1;
+                    union.union(pairToIndex((j,i), dim), pairToIndex((j,i+1), dim));
+                }
+                if j+1 < dim.0 && data[i][j] == data[i][j+1] {
+                    pairToIndexLess((j,i), dim);
+                    pairToIndexLess((j+1,i), dim);
+                    assert union.parent.Length == dim.0 * dim.1;
+                    union.union(pairToIndex((j,i), dim), pairToIndex((j+1,i), dim));
+                }
+            }
+        }
+        var groupings: map<nat, seq<(nat, nat)>> := map[];
+        for i := 0 to dim.0 * dim.1 
+            invariant union.n == dim.0 * dim.1
+            invariant union.Valid()
+            invariant forall key :: key in groupings.Keys ==> forall x :: x in groupings[key] ==> 0 <= x.0 < dim.0 && 0 <= x.1 < dim.1
+            modifies union.parent
+        {
+            var root := union.findRoot(i);
+            if root !in groupings {
+                groupings := groupings[root := [indexToPair(i, dim)]];
+            } else {
+                groupings := groupings[root := groupings[root] + [indexToPair(i, dim)]];
+            }
+        }
+        var groups := groupings.Keys;
+        var what := groupings.Values;
+        while groups != {} {
+            var group :| group in groups;
+            var groupMembers := groupings[group];
+            groups := groups - {group};
+            var perimeter := 0;
+            for i := 0 to |groupMembers| {
+                var p: (nat, nat) := groupMembers[i];
+                if (0 <= (p.0-1 as int) && data[p.1][p.0-1] != data[p.1][p.0]) || p.0 == 0 {
+                    perimeter := perimeter + 1;
+                }
+                if (p.0+1 < dim.0 && data[p.1][p.0+1] != data[p.1][p.0]) || p.0 == dim.0-1 {
+                    perimeter := perimeter + 1;
+                }
+                if (0 <= p.1-1 && data[p.1-1][p.0] != data[p.1][p.0]) || p.1 == 0 {
+                    perimeter := perimeter + 1;
+                }
+                if (p.1+1 < dim.1 && data[p.1+1][p.0] != data[p.1][p.0]) || p.1 == dim.1-1 {
+                    perimeter := perimeter + 1;
+                }
+            }
+            x := x + perimeter * |groupMembers|;
+        }
+
     }
 
     method problem12_2(input: string) returns (x: int) {
