problems/12/QuickUnion.dfy
@@ -1,0 +1,98 @@
+
+module QuickUnion {
+
+
+    class QuickUnion {
+        var n : nat
+        var parent: array<nat>
+        var size: array<nat>
+
+        constructor(n: nat) 
+            requires n > 0
+            ensures this.n == n
+            ensures this.parent.Length == this.n
+            ensures this.size.Length == this.n
+            ensures fresh(this)
+            ensures Valid()
+        {
+            parent := new nat[n];
+            size := new nat[n];
+            this.n := n;
+            new;
+            assert parent.Length == n;
+            assert size.Length == n;
+            forall i | 0 <= i < n {
+                parent[i] := i;
+            }
+            forall i | 0 <= i < n {
+                size[i] := 1;
+            }
+        }
+
+        predicate Valid()
+            reads this, parent, size
+        {
+            this.parent.Length > 0 &&
+            this.parent.Length == this.size.Length == this.n &&
+            this.parent != this.size &&
+            (forall i :: 0 <= i < this.parent.Length ==> 0 <= parent[i] < parent.Length)
+            && (forall i :: 0 <= i < this.size.Length ==> this.size[i] > 0)
+        }
+
+        method findRoot(x: nat) returns (root: nat)
+            requires Valid()
+            requires 0 <= x < parent.Length
+            ensures 0 <= root < parent.Length
+            ensures parent.Length == old(parent.Length)
+            ensures Valid()
+            modifies parent
+            decreases *
+        {
+            root := x;
+            // ghost var all := multiset(parent[..]);
+            // ghost var visited: set<nat> := {};
+            while root != parent[root]
+                invariant Valid()
+                invariant 0 <= root < parent.Length
+                decreases *
+            {
+                root := parent[root];
+            }
+            this.parent[x] := root;
+        }
+
+        method connected(x: nat, y: nat) returns (result: bool)
+            requires 0 <= x < parent.Length
+            requires 0 <= y < parent.Length
+            requires Valid()
+            decreases *
+            modifies parent
+            ensures Valid()
+        {
+            var xroot := this.findRoot(x);
+            var yroot := this.findRoot(y);
+            result := xroot == yroot;
+        }
+
+        method union(x: nat, y: nat)
+            requires 0 <= x < parent.Length
+            requires 0 <= y < parent.Length
+            requires Valid()
+            decreases *
+            modifies parent, size
+            ensures Valid()
+        {
+            var rootX := findRoot(x);
+            var rootY := findRoot(y);
+            if rootX != rootY {
+                if size[rootX] < size[rootY] {
+                    size[rootY] := size[rootY] + size[rootX];
+                    parent[rootX] := rootY;
+                } else {
+                    size[rootX] := size[rootX] + size[rootY];
+                    parent[rootY] := rootX;
+                }
+            }
+        }
+    }
+}
